change abstract ES array functions
to work on CArrPtr arguments instead of CArrES arguments

isa/Gencot_ESArray_Lemmas.thy
@@ -11,23 +11,23 @@ consts
 
 text \<open>Define the abstract data type functions for explicitly sized arrays.
 The explicit size is ignored and the intrinsic size of the list is used.\<close>
-definition sizES :: "'el CArrES\<^sub>T \<Rightarrow> nat"
-  where "sizES a \<equiv> length (fst a)"
-definition vldES :: "'el CArrES\<^sub>T \<Rightarrow> nat \<Rightarrow> bool"
+definition sizES :: "'el CArrPtr\<^sub>T \<Rightarrow> nat"
+  where sizES_def[simp]: "sizES a \<equiv> length a"
+definition vldES :: "'el CArrPtr\<^sub>T \<Rightarrow> nat \<Rightarrow> bool"
   where "vldES a i \<equiv> i < sizES a"
-definition elmES :: "nat \<Rightarrow> 'el CArrES\<^sub>T \<Rightarrow> 'el"
-  where "elmES i a \<equiv> nth (fst a) i"
-definition elm_updateES :: "nat \<Rightarrow> ('el \<Rightarrow> 'el) \<Rightarrow> 'el CArrES\<^sub>T \<Rightarrow> 'el CArrES\<^sub>T"
-  where "elm_updateES i f a \<equiv> ((list_update (fst a) i (f (elmES i a))),snd a)"
-definition elm_modifiedES :: "nat \<Rightarrow> ('el \<Rightarrow> 'el \<Rightarrow> bool) \<Rightarrow> 'el CArrES\<^sub>T \<Rightarrow> 'el CArrES\<^sub>T \<Rightarrow> bool"
+definition elmES :: "nat \<Rightarrow> 'el CArrPtr\<^sub>T \<Rightarrow> 'el"
+  where "elmES i a \<equiv> nth a i"
+definition elm_updateES :: "nat \<Rightarrow> ('el \<Rightarrow> 'el) \<Rightarrow> 'el CArrPtr\<^sub>T \<Rightarrow> 'el CArrPtr\<^sub>T"
+  where "elm_updateES i f a \<equiv> (list_update a i (f (elmES i a)))"
+definition elm_modifiedES :: "nat \<Rightarrow> ('el \<Rightarrow> 'el \<Rightarrow> bool) \<Rightarrow> 'el CArrPtr\<^sub>T \<Rightarrow> 'el CArrPtr\<^sub>T \<Rightarrow> bool"
   where elm_modified_def: "elm_modifiedES i m a1 a2 \<equiv> 
     m (elmES i a1) (elmES i a2) \<and> (\<forall>j \<noteq> i. vldES a1 j \<longrightarrow> elmES j a1 = elmES j a2)"
-definition arr_fill_nES :: "nat \<Rightarrow> (nat \<Rightarrow> 'el) \<Rightarrow> 'el CArrES\<^sub>T"
-  where "arr_fill_nES n f \<equiv> ([f x . x \<leftarrow> [0 ..< n]],of_nat n)"
+definition arr_fill_nES :: "nat \<Rightarrow> (nat \<Rightarrow> 'el) \<Rightarrow> 'el CArrPtr\<^sub>T"
+  where "arr_fill_nES n f \<equiv> [f x . x \<leftarrow> [0 ..< n]]"
 
 text \<open>Laws for the abstract data type functions\<close>
-lemma vldArrES: "vldES a n = (n < length (fst a))"
-  by (simp add: vldES_def sizES_def)
+lemma vldArrES: "vldES a n = (n < length a)"
+  by (simp add: vldES_def)
 lemma elm_identUpdES[simp]: "elm_updateES i (\<lambda>a. a) = (\<lambda>a. a)"
   apply (unfold elm_updateES_def)
   by(simp add: elmES_def)
@@ -35,7 +35,7 @@ lemma elm_sameUpdES: "elm_updateES i (\<lambda>_. m (elmES i x)) x = elm_updateE
   by(simp add: elm_updateES_def)
 thm list_update_same_conv
 lemma elm_distUpdES: "vldES a i \<Longrightarrow> (elm_updateES i f) ( (elm_updateES i g) a) = elm_updateES i (f \<circ> g) a"
-  for f:: "'el \<Rightarrow> 'el" and a::"'el CArrES\<^sub>T"
+  for f:: "'el \<Rightarrow> 'el" and a::"'el CArrPtr\<^sub>T"
   apply (unfold elm_updateES_def elmES_def fst_def vldArrES)
   by(auto)
 lemma elm_commUpd_elmES: "i < j \<Longrightarrow> (elm_updateES j m2) \<circ> (elm_updateES i m1) = (elm_updateES i m1) \<circ> (elm_updateES j m2)"
@@ -49,36 +49,37 @@ lemma elmElmUpdFrameES: "vldES a i \<and> vldES a j \<and> i \<noteq> j \<Longri
   by(auto simp add: elm_updateES_def elmES_def vldArrES)
 lemma elmArrFillES: "i < n \<Longrightarrow> elmES i (arr_fill_nES n f) = f i"
   by(auto simp add: elmES_def arr_fill_nES_def vldArrES)
+lemma sizArrFill: "sizES (arr_fill_nES n f) = n"
+  by(auto simp add: arr_fill_nES_def)
 
 text \<open>Array equality by extensionality. \<close>
-lemma eqArrES: "snd a1 = snd a2 \<Longrightarrow> sizES a1 = sizES a2 \<Longrightarrow>
+lemma eqArrES: "sizES a1 = sizES a2 \<Longrightarrow>
               (a1 = a2) = 
               (\<forall> i. (vldES a1 i) \<longrightarrow> ((elmES i a1) = (elmES i a2)))"
-  for a1::"'el CArrES\<^sub>T" and a2::"'el CArrES\<^sub>T"
+  for a1::"'el CArrPtr\<^sub>T" and a2::"'el CArrPtr\<^sub>T"
   apply(rule iffI)
    apply(rule allI)
    apply(rule impI)
-   apply(auto simp add: elmES_def vldArrES sizES_def)
+   apply(auto simp add: elmES_def vldArrES)
   apply(case_tac a1)
   apply(case_tac a2)
   apply(auto)
   apply(rule nth_equalityI)
   by(auto)
 
-lemma eqElmUpdES: "sizES a1 = sizES a2 \<Longrightarrow> snd a1 = snd a2 \<Longrightarrow> vldES a2 i \<Longrightarrow> (a1 = elm_updateES i f a2) =
+lemma eqElmUpdES: "sizES a1 = sizES a2 \<Longrightarrow> vldES a2 i \<Longrightarrow> (a1 = elm_updateES i f a2) =
                  ((elmES i a1) = f (elmES i a2) \<and> (\<forall> j. j \<noteq> i \<and> (vldES a1 j) \<longrightarrow> (elmES j a1) = (elmES j a2)))"
   apply(rule iffI)
    apply(auto)
     apply(subst elmElmUpdES,auto)
-  apply(subst elmElmUpdFrameES,auto simp add: vldArrES sizES_def)
+  apply(subst elmElmUpdFrameES,auto simp add: vldArrES)
   apply(subst eqArrES)
     apply(auto simp add:elm_updateES_def)
-   apply(auto simp add: sizES_def)
    apply(auto simp add: elmES_def)
   apply(case_tac "ia = i")
    apply(simp)
   by(auto simp add: vldArrES)
-lemma eqArrFillES: "sizES a = n \<Longrightarrow> snd a = of_nat n \<Longrightarrow> (a = arr_fill_nES n f) = 
+lemma eqArrFillES: "sizES a = n \<Longrightarrow> (a = arr_fill_nES n f) = 
                  ((\<forall> i. (vldES a i) \<longrightarrow> ((elmES i a) = f i)))"
   apply(rule iffI)
    apply(auto)
@@ -86,11 +87,10 @@ lemma eqArrFillES: "sizES a = n \<Longrightarrow> snd a = of_nat n \<Longrightar
    apply(simp add: vldArrES arr_fill_nES_def)
   apply(subst eqArrES)
    apply(simp add: vldArrES arr_fill_nES_def)
-   apply(simp add: sizES_def arr_fill_nES_def)
+   apply(simp add: arr_fill_nES_def)
    apply(rule allI)
    apply(rule impI)
-  apply(subst elmArrFillES)
-  by (auto simp add: vldArrES sizES_def)
+  by (auto simp add: elmES_def vldArrES)
 
 text \<open>Semantics theorems for the Gencot array functions.\<close>
 
@@ -99,7 +99,7 @@ definition ctrct_getArrES :: "'el CArrES\<^sub>T \<times> ('m::len) word \<Right
   "ctrct_getArrES x \<equiv> let ((a,n),i) = x in unat n = length a \<and> (unat i) < (unat n)"
 theorem sem_getArrES[sem]: 
  "ctrct_getArrES (a,i) \<Longrightarrow> 
-  getArrES (a,i) = elmES (unat i) a"
+  getArrES (a,i) = elmES (unat i) (fst a)"
   by (auto simp add: getArrES_def elmES_def)
 
 definition ctrct_setArrES :: "'el CArrES\<^sub>T \<times> ('m::len) word \<times> 'el \<Rightarrow> bool"
@@ -107,7 +107,7 @@ definition ctrct_setArrES :: "'el CArrES\<^sub>T \<times> ('m::len) word \<times
   "ctrct_setArrES x \<equiv> let ((a,n),i,v) = x in unat n = length a \<and> (unat i) < (unat n)"
 theorem sem_setArrES[sem]: 
  "ctrct_setArrES (a,i,v) \<Longrightarrow> 
-  setArrES (a,i,v) = (elm_updateES (unat i) (\<lambda>_.v) a, ())"
+  setArrES (a,i,v) = ((elm_updateES (unat i) (\<lambda>_.v) (fst a),(snd a)), ())"
   by (auto simp add: setArrES_def elm_updateES_def)
 
 definition ctrct_modifyArrES :: "'el CArrES\<^sub>T \<times> ('m::len) word \<times> ('el \<times> 'arg \<Rightarrow> 'el \<times> 'arg) \<times> 'arg \<Rightarrow> bool"
@@ -116,7 +116,8 @@ definition ctrct_modifyArrES :: "'el CArrES\<^sub>T \<times> ('m::len) word \<ti
 theorem sem_modifyArrES[sem]:
  "ctrct_modifyArrES (a,i,f,x) \<Longrightarrow> 
   modifyArrES (a,i,f,x) = 
-  (let (e,y) = f (elmES (unat i) a, x) in (elm_updateES (unat i) (\<lambda>_.e) a, y))"
+  (let (e,y) = f (elmES (unat i) (fst a), x) 
+  in ((elm_updateES (unat i) (\<lambda>_.e) (fst a),(snd a)), y))"
   by (simp add: modifyArrES_def split_def Let_def elm_updateES_def elmES_def)
 
 definition ctrct_modifyArrDfltES :: "'el CArrES\<^sub>T \<times> ('m::len) word \<times> ('el \<times> 'arg \<Rightarrow> 'el \<times> 'out) \<times> 'arg \<Rightarrow> bool"
@@ -125,7 +126,8 @@ definition ctrct_modifyArrDfltES :: "'el CArrES\<^sub>T \<times> ('m::len) word 
 theorem sem_modifyArrDfltES[sem]:
  "ctrct_modifyArrDfltES (a,i,f,x) ==> 
   modifyArrDfltES (a,i,f,x) = 
-  (let (e,y) = f (elmES (unat i) a, x) in (elm_updateES (unat i) (\<lambda>_.e) a, y))"
+  (let (e,y) = f (elmES (unat i) (fst a), x) 
+  in ((elm_updateES (unat i) (\<lambda>_.e) (fst a),(snd a)), y))"
   by (simp add: modifyArrDfltES_def split_def Let_def elm_updateES_def elmES_def)
 
 definition ctrct_modrefArrES :: "'el CArrES\<^sub>T \<times> ('m::len) word \<times> ('pel \<times> 'arg \<Rightarrow> 'pel \<times> 'arg) \<times> 'arg \<Rightarrow> bool"
@@ -134,7 +136,8 @@ definition ctrct_modrefArrES :: "'el CArrES\<^sub>T \<times> ('m::len) word \<ti
 theorem sem_modrefArrES[sem]:
  "ctrct_modrefArrES (a,i,f,x) \<Longrightarrow> 
   modrefArrES (a,i,f,x) = 
-  (let (e,y) = f (toPtr (elmES (unat i) a), x) in (elm_updateES (unat i) (\<lambda>_.frPtr e) a, y))"
+  (let (e,y) = f (toPtr (elmES (unat i) (fst a)), x) 
+  in ((elm_updateES (unat i) (\<lambda>_.frPtr e) (fst a),(snd a)), y))"
   by (simp add: modrefArrES_def split_def Let_def elm_updateES_def elmES_def)
 
 definition ctrct_modrefArrDfltES :: "'el CArrES\<^sub>T \<times> ('m::len) word \<times> ('pel \<times> 'arg \<Rightarrow> 'pel \<times> 'out) \<times> 'arg \<Rightarrow> bool"
@@ -143,7 +146,8 @@ definition ctrct_modrefArrDfltES :: "'el CArrES\<^sub>T \<times> ('m::len) word 
 theorem sem_modrefArrDfltES[sem]:
  "ctrct_modrefArrDfltES (a,i,f,x) ==> 
   modrefArrDfltES (a,i,f,x) = 
-  (let (e,y) = f (toPtr (elmES (unat i) a), x) in (elm_updateES (unat i) (\<lambda>_.frPtr e) a, y))"
+  (let (e,y) = f (toPtr (elmES (unat i) (fst a)), x) 
+  in ((elm_updateES (unat i) (\<lambda>_.frPtr e) (fst a),(snd a)), y))"
   by (simp add: modrefArrDfltES_def split_def Let_def elm_updateES_def elmES_def)
 
 end
